back to a more standard disk abstraction
Implement a more traditional-looking log, without a special "log" sector
content type, by using the first 5 disk sectors to store the log.

Proof that log works without crashes starting from a clean disk is OK.
Other proofs seem more complicated, and the rewrite_disk_ops Ltac is
getting way too messy.

coqfs.v
@@ -2,20 +2,20 @@ Require Import Arith.
 Require Import CpdtTactics.
 
 Inductive diskblock :=
-  | Data : forall (data:nat), diskblock
-  | Log : forall (addr0:nat) (data0:nat) (addr1:nat) (data1:nat), diskblock
-  | EmptyLog : diskblock.
+  | Data : nat -> diskblock.
 
 Definition disk := nat -> diskblock.
 
 Definition empty_disk : disk :=
   fun n => Data 0.
 
-Definition disk_write (addr:nat) (val:diskblock) (d:disk) : disk :=
-  fun n => if eq_nat_dec n addr then val else d n.
+Definition disk_write (addr:nat) (val:nat) (d:disk) : disk :=
+  fun n => if eq_nat_dec n addr then Data val else d n.
 
-Definition disk_read (addr:nat) (d:disk) : diskblock :=
-  d addr.
+Definition disk_read (addr:nat) (d:disk) : nat :=
+  match d addr with
+  | Data n => n
+  end.
 
 
 Inductive flaky_disk :=
@@ -30,14 +30,14 @@ Definition flaky_fix (fd:flaky_disk) : flaky_disk :=
   | GoodDisk d => GoodDisk d
   end.
 
-Definition flaky_write (addr:nat) (val:diskblock) (fd:flaky_disk) : flaky_disk :=
+Definition flaky_write (addr:nat) (val:nat) (fd:flaky_disk) : flaky_disk :=
   match fd with
   | FlakyDisk _ 0 => fd
   | FlakyDisk d (S k) => FlakyDisk (disk_write addr val d) k
   | GoodDisk d => GoodDisk (disk_write addr val d)
   end.
 
-Definition flaky_read (addr:nat) (fd:flaky_disk) : diskblock :=
+Definition flaky_read (addr:nat) (fd:flaky_disk) : nat :=
   match fd with
   | FlakyDisk d _ => disk_read addr d
   | GoodDisk d => disk_read addr d
@@ -45,16 +45,14 @@ Definition flaky_read (addr:nat) (fd:flaky_disk) : diskblock :=
 
 
 Definition inc (addr:nat) (fd:flaky_disk) : flaky_disk :=
-  match flaky_read addr fd with
-  | Data x => flaky_write addr (Data (x+1)) fd
-  | _ => fd
-  end.
+  let old := flaky_read addr fd in
+  flaky_write addr (old+1) fd.
 
 
 Theorem inc_ok:
   forall fd fd' addr k,
-  flaky_read addr fd = Data k /\ inc addr fd = fd' ->
-  flaky_read addr fd = Data k \/ flaky_read addr fd = Data (k+1).
+  flaky_read addr fd = k /\ inc addr fd = fd' ->
+  flaky_read addr fd = k \/ flaky_read addr fd = (k+1).
 Proof.
   crush.
 Qed.
@@ -62,32 +60,38 @@ Qed.
 
 Definition log_apply (fd:flaky_disk) : flaky_disk :=
   match flaky_read 0 fd with
-  | Log a0 d0 a1 d1 =>
-    flaky_write 0 EmptyLog (flaky_write a0 (Data d0) (flaky_write a1 (Data d1) fd))
-  | _ => fd
-  end.
-
-Definition block_inc (b:diskblock) : nat :=
-  match b with
-  | Data x => x+1
-  | _ => 0
+  | 0 => fd
+  | S _ =>
+    let a0 := flaky_read 1 fd in
+    let a1 := flaky_read 2 fd in
+    let d0 := flaky_read 3 fd in
+    let d1 := flaky_read 4 fd in
+    flaky_write 0 0 (flaky_write a0 d0 (flaky_write a1 d1 fd))
   end.
 
 Definition log_doubleinc (addr:nat) (fd:flaky_disk) : flaky_disk :=
   let fd0 := log_apply fd in
-  let d0 := flaky_read (addr+1) fd0 in
-  let d1 := flaky_read (addr+2) fd0 in
-  let fd1 := flaky_write 0 (Log (addr+1) (block_inc d0)
-                                (addr+2) (block_inc d1)) fd0 in
+  let d0 := flaky_read (addr+5) fd0 in
+  let d1 := flaky_read (addr+6) fd0 in
+  let fd1 := flaky_write 0 1
+            (flaky_write 1 (addr+5)
+            (flaky_write 2 (addr+6)
+            (flaky_write 3 (d0+1)
+            (flaky_write 4 (d1+1) fd0)))) in
   log_apply fd1.
 
 Definition log_read (addr:nat) (fd:flaky_disk) : nat :=
   let fd0 := log_apply fd in
-  match flaky_read (S addr) fd0 with
-  | Data x => x
-  | _ => 0
-  end.
+  flaky_read (addr+5) fd0.
 
+
+Lemma disk_read_eq:
+  forall d a x,
+  disk_read a (disk_write a x d) = x.
+Proof.
+  intros; unfold disk_read; unfold disk_write.
+  destruct (eq_nat_dec a a); crush.
+Qed.
 
 Lemma disk_read_same:
   forall d a a' x,
@@ -112,12 +116,20 @@ Qed.
  *)
 Ltac rewrite_disk_ops :=
   simpl;
+  repeat (rewrite disk_read_eq in *);
   repeat (rewrite disk_read_other with (a:=S _) (a':=0) in *; [idtac|crush]);
   repeat (rewrite disk_read_other with (a:=_+1) (a':=0) in *; [idtac|crush]);
   repeat (rewrite disk_read_other with (a:=_+2) (a':=0) in *; [idtac|crush]);
   repeat (rewrite disk_read_other with (a:=0) (a':=S _) in *; [idtac|crush]);
   repeat (rewrite disk_read_other with (a:=0) (a':=_+1) in *; [idtac|crush]);
   repeat (rewrite disk_read_other with (a:=0) (a':=_+2) in *; [idtac|crush]);
+  repeat (rewrite disk_read_other with (a:=1) (a':=2) in *; [idtac|crush]);
+  repeat (rewrite disk_read_other with (a:=2) (a':=1) in *; [idtac|crush]);
+  repeat (rewrite disk_read_other with (a:=3) (a':=1) in *; [idtac|crush]);
+  repeat (rewrite disk_read_other with (a:=3) (a':=2) in *; [idtac|crush]);
+  repeat (rewrite disk_read_other with (a:=4) (a':=1) in *; [idtac|crush]);
+  repeat (rewrite disk_read_other with (a:=4) (a':=2) in *; [idtac|crush]);
+  repeat (rewrite disk_read_other with (a:=4) (a':=3) in *; [idtac|crush]);
   repeat (rewrite disk_read_same with (a:=S (_+1)) (a':=_+2) in *; [idtac|crush]);
   repeat (rewrite disk_read_other with (a:=S _) (a':=_+2) in *; [idtac|crush]);
   repeat (rewrite disk_read_other with (a:=S (_+1)) (a':=_+1) in *; [idtac|crush]);
@@ -126,7 +138,13 @@ Ltac rewrite_disk_ops :=
   repeat (rewrite disk_read_same with (a:=0) (a':=0) in *; [idtac|crush]);
   repeat (rewrite disk_read_same with (a:=S _) (a':=_+1) in *; [idtac|crush]);
   repeat (rewrite disk_read_other with (a:=_+1) (a':=_+2) in *; [idtac|crush]);
-  repeat (rewrite disk_read_other with (a:=_+2) (a':=_+1) in *; [idtac|crush]).
+  repeat (rewrite disk_read_other with (a:=_+2) (a':=_+1) in *; [idtac|crush]);
+  repeat (rewrite disk_read_other with (a:=_+5) (a':=0) in *; [idtac|crush]);
+  repeat (rewrite disk_read_same with (a:=_+1+5) (a':=_+1+5) in *; [idtac|crush]);
+  repeat (rewrite disk_read_same with (a:=_+1+5) (a':=_+6) in *; [idtac|crush]);
+  repeat (rewrite disk_read_other with (a:=_+5) (a':=_+1+5) in *; [idtac|crush]);
+  repeat (rewrite disk_read_other with (a:=_+1+5) (a':=_+5) in *; [idtac|crush]);
+  repeat (rewrite disk_read_same with (a:=_+5) (a':=_+5) in *; [idtac|crush]).
 
 Theorem doubleinc_init_nocrash:
   forall fd addr,
@@ -145,6 +163,19 @@ Proof.
   repeat rewrite_disk_ops; auto.
 Qed.
 
+Theorem doubleinc_nocrash:
+  forall fd' fd addr a b,
+  flaky_read 0 fd' = 0 ->
+  log_read addr     fd' = a ->
+  log_read (addr+1) fd' = b ->
+  log_doubleinc addr (flaky_fix fd') = fd ->
+  log_read addr     fd = (a+1) /\
+  log_read (addr+1) fd = (b+1).
+Proof.
+  (* XXX *)
+Abort.
+
+(*
 Theorem doubleinc_init_crash:
   forall n fd addr,
   log_doubleinc addr (flaky_init empty_disk n) = fd ->
@@ -182,3 +213,10 @@ Proof.
   repeat rewrite_disk_ops; auto.
 Qed.
 
+Theorem log_apply_crash:
+  forall fd,
+  log_apply (flaky_fix (log_apply fd)) = log_apply (flaky_fix fd).
+Proof.
+  (* XXX *)
+Abort.
+*)
